WIP write_expr_base

tests/pulse/ArithParse.Impl.fst
@@ -21,8 +21,8 @@ let validate_header_rhs (lhs: U8.t) : validator (parse_header_rhs lhs) =
   ifthenelse_validator
     (parse_header_rhs lhs)
     (lhs = 255uy)
-    (fun _ -> validate_weaken parse_header_rhs_kind (validate_u64))
-    (fun _ -> validate_weaken parse_header_rhs_kind (validate_ret u_as_uint64))
+    (fun _ -> validate_weaken parse_header_rhs_kind (validate_synth (validate_u64) (HValue #lhs ())))
+    (fun _ -> validate_weaken parse_header_rhs_kind (validate_synth validate_empty (HUnit #lhs ())))
 
 inline_for_extraction noextract [@@noextract_to "krml"]
 let validate_header : validator parse_header =
@@ -33,12 +33,24 @@ let jump_header_rhs (lhs: U8.t) : jumper (parse_header_rhs lhs) =
   ifthenelse_jumper
     (parse_header_rhs lhs)
     (lhs = 255uy)
-    (fun _ -> jump_ext (jump_u64) (parse_header_rhs lhs))
-    (fun _ -> jump_ext (jump_ret u_as_uint64) (parse_header_rhs lhs))
+    (fun _ -> jump_ext (jump_synth jump_u64 (HValue #lhs ())) (parse_header_rhs lhs))
+    (fun _ -> jump_ext (jump_synth jump_empty (HUnit #lhs ())) (parse_header_rhs lhs))
 
 inline_for_extraction noextract [@@noextract_to "krml"]
 let jump_header : jumper parse_header =
   jump_dtuple2 jump_u8 (leaf_reader_of_reader read_u8) jump_header_rhs
+
+let write_header : l2r_leaf_writer serialize_header =
+  l2r_leaf_write_dtuple2
+    (l2r_leaf_write_u8 ())
+    ()
+    (fun lhs ->
+      l2r_leaf_writer_ifthenelse
+        (serialize_header_rhs lhs)
+        (lhs = 255uy)
+        (fun _ -> l2r_leaf_writer_ext (l2r_leaf_write_synth' (l2r_leaf_write_u64 ()) (HValue ()) (HValue?.v)) (serialize_header_rhs lhs))
+        (fun _ -> l2r_leaf_writer_ext (l2r_leaf_write_synth' (l2r_leaf_write_empty) (HUnit ()) (HUnit?.v)) (serialize_header_rhs lhs))
+    )
 
 module SZ = FStar.SizeT
 
@@ -110,43 +122,18 @@ let jump_expr : jumper tot_parse_expr =
 (* Low-level data structure *)
 
 noeq
-type expr_t =
-| EUnparsed of with_perm (S.slice U8.t)
-| EPlus of with_perm (S.slice expr_t)
-| EMinus of (with_perm (ref expr_t) & with_perm (ref expr_t))
+type expr_base_t =
+| EUPlus: (count: U8.t) -> (payload: with_perm (S.slice U8.t)) -> expr_base_t
+| EUMinus: (fst: with_perm (S.slice U8.t)) -> (snd: with_perm (S.slice U8.t)) -> expr_base_t
 | EValue of U64.t
 
+noeq
+type expr_t =
+| EBase of expr_base_t // or value
+| EPlus of with_perm (S.slice expr_t)
+| EMinus: (fst: with_perm (ref expr_t)) -> (snd: with_perm (ref expr_t)) -> expr_t
+
 (* Separation-logic predicate *)
-
-let nlist_match_slice0
-  (#telem: Type0)
-  (#t: Type)
-  (vmatch: (telem -> t -> slprop))
-= nlist_match_slice Some (fun _ -> vmatch)
-
-let nlist_match_slice_wf
-  (#telem: Type0)
-  (#t: Type)
-  (n: nat)
-  (a: _)
-  (l: LowParse.Spec.VCList.nlist n t)
-  (vmatch: (telem -> (x: t { x << l }) -> slprop))
-: Tot slprop
-= exists* (ar: with_perm (S.slice telem)) c .
-    pts_to ar.v #ar.p c **
-    PM.seq_list_match c l (vmatch) **
-    pure (Some a == Some ar)
-
-let nlist_match_slice_wf_eq
-  (#telem: Type0)
-  (#t: Type)
-  (vmatch: (telem -> t -> slprop))
-  (n: nat)
-  (a: _)
-  (l: LowParse.Spec.VCList.nlist n t)
-: Lemma
-  (nlist_match_slice0 vmatch n a l == nlist_match_slice_wf n a l vmatch)
-= assert_norm (nlist_match_slice0 vmatch n a l == nlist_match_slice_wf n a l vmatch)
 
 let vmatch_pair
   (#tl1 #tl2 #th1 #th2: Type)
@@ -156,6 +143,26 @@ let vmatch_pair
   (xh: (th1 & th2))
 : Tot slprop
 = vmatch1 (fst xl) (fst xh) ** vmatch2 (snd xl) (snd xh)
+
+[@@pulse_unfold]
+let rel_base_EUPlus
+  (count: U8.t)
+  (pl: with_perm (S.slice U8.t))
+  (n: nat)
+  (sq: squash (n < 254))
+  (l: nlist n expr)
+: Tot slprop
+= vmatch_and_const (pure (eq2 #nat n (U8.v count))) (pts_to_serialized_with_perm (serialize_nlist n serialize_expr)) pl l // FIXME: WHY WHY WHY WHY WHY WHY do I need this F*ing annotation on eq2? I wasted HOURS on this
+
+let rel_base
+  (base: expr_base_t)
+  (e: expr)
+: Tot slprop
+= match base, e with
+  | EUPlus count pl, Plus n sq l -> rel_base_EUPlus count pl n sq l
+  | EUMinus fst snd, Minus v -> vmatch_pair (pts_to_serialized_with_perm serialize_expr) (pts_to_serialized_with_perm serialize_expr) (fst, snd) v
+  | EValue vl, Value vh -> eq_as_slprop U64.t vl vh
+  | _ -> pure False
 
 let vmatch_ref
   (#tl #th: Type0)
@@ -210,10 +217,9 @@ let rec rel
 : Tot slprop
   (decreases high)
 = match low, high with
-  | EUnparsed s, _ -> pts_to_serialized_with_perm (serializer_of_tot_serializer tot_serialize_expr) s high
-  | EPlus s, Plus l -> nlist_match_slice_wf (List.Tot.length l) s l rel
-  | EMinus pl, Minus ph -> vmatch_pair (vmatch_ref_wf (Minus ph) rel) (vmatch_ref_wf (Minus ph) rel) pl ph
-  | EValue vl, Value vh -> eq_as_slprop U64.t vl vh
+  | EBase vb, l -> rel_base vb l
+  | EPlus s, Plus n _ l -> nlist_match_slice_wf n s l rel
+  | EMinus pl1 pl2, Minus ph -> vmatch_pair (vmatch_ref_wf (Minus ph) rel) (vmatch_ref_wf (Minus ph) rel) (pl1, pl2) ph
   | _ -> pure False
 
 let rel'
@@ -222,10 +228,9 @@ let rel'
 : Tot slprop
   (decreases high)
 = match low, high with
-  | EPlus s, Plus l -> nlist_match_slice0 rel (List.Tot.length l) s l
-  | EMinus pl, Minus ph -> vmatch_pair (vmatch_ref rel) (vmatch_ref rel) pl ph
-  | EValue vl, Value vh -> eq_as_slprop U64.t vl vh
-  | EUnparsed s, _ -> pts_to_serialized_with_perm (serializer_of_tot_serializer tot_serialize_expr) s high
+  | EBase vb, l -> rel_base vb l
+  | EPlus s, Plus n _ l -> nlist_match_slice0 rel n s l
+  | EMinus pl1 pl2, Minus ph -> vmatch_pair (vmatch_ref rel) (vmatch_ref rel) (pl1, pl2) ph
   | _ -> pure False
 
 let rel_eq
@@ -234,20 +239,47 @@ let rel_eq
 : Lemma
   (rel low high == rel' low high)
 = match low, high with
-  | EPlus s, Plus l ->
-    assert_norm (rel (EPlus s) (Plus l) == nlist_match_slice_wf (List.Tot.length l) s l (rel));
-    assert_norm (rel' (EPlus s) (Plus l) == nlist_match_slice0 rel (List.Tot.length l) s l);
-    nlist_match_slice_wf_eq (rel) (List.Tot.length l) s l;
+  | EPlus s, Plus n _ l ->
+    assert_norm (rel (EPlus s) (Plus n _ l) == nlist_match_slice_wf n s l (rel));
+    assert_norm (rel' (EPlus s) (Plus n _ l) == nlist_match_slice0 rel n s l);
+    nlist_match_slice_wf_eq (rel) n s l;
     ()
-  | EMinus pl, Minus ph ->
-    assert (rel (EMinus pl) (Minus ph) == vmatch_pair (vmatch_ref_wf (Minus ph) rel) (vmatch_ref_wf (Minus ph) rel) pl ph) by (FStar.Tactics.trefl ());
-    assert (rel' (EMinus pl) (Minus ph) == vmatch_pair (vmatch_ref rel) (vmatch_ref rel) pl ph) by (FStar.Tactics.trefl ());
-    vmatch_ref_wf_eq (Minus ph) rel (fst pl) (fst ph);
-    vmatch_ref_wf_eq (Minus ph) rel (snd pl) (snd ph);
+  | EMinus pl1 pl2, Minus ph ->
+    assert (rel (EMinus pl1 pl2) (Minus ph) == vmatch_pair (vmatch_ref_wf (Minus ph) rel) (vmatch_ref_wf (Minus ph) rel) (pl1, pl2) ph) by (FStar.Tactics.trefl ());
+    assert (rel' (EMinus pl1 pl2) (Minus ph) == vmatch_pair (vmatch_ref rel) (vmatch_ref rel) (pl1, pl2) ph) by (FStar.Tactics.trefl ());
+    vmatch_ref_wf_eq (Minus ph) rel (pl1) (fst ph);
+    vmatch_ref_wf_eq (Minus ph) rel (pl2) (snd ph);
     ()
   | _ -> ()
 
 // from now on, rel should be opaque
+
+let rel_base_cases_bool
+  (low: expr_base_t)
+  (high: expr)
+: GTot bool
+  (decreases high)
+= match low, high with
+  | EUPlus _ _, Plus _ _ _
+  | EUMinus _ _, Minus _
+  | EValue _, Value _
+    -> true
+  | _ -> false
+
+ghost fn rel_base_cases
+  (low: expr_base_t)
+  (high: expr)
+requires rel_base low high
+ensures rel_base low high ** pure (rel_base_cases_bool low high == true)
+{
+  let g = rel_base_cases_bool low high;
+  if (g) {
+    ()
+  } else {
+    rewrite (rel_base low high) as (pure False);
+    rewrite (pure False) as (rel_base low high)
+  }
+}
 
 let rel_cases_bool
   (low: expr_t)
@@ -255,10 +287,9 @@ let rel_cases_bool
 : GTot bool
   (decreases high)
 = match low, high with
-  | EPlus _, Plus _
-  | EMinus _, Minus _
-  | EValue _, Value _
-  | EUnparsed _, _ -> true
+  | EPlus _, Plus _ _ _
+  | EMinus _ _, Minus _
+  | EBase _, _ -> true
   | _ -> false
 
 ghost fn rel_cases
@@ -273,5 +304,167 @@ ensures rel low high ** pure (rel_cases_bool low high == true)
   } else {
     rewrite (rel low high) as (pure False);
     rewrite (pure False) as (rel low high)
+  }
+}
+
+ghost
+fn rewrite_with_trade_squash
+  (#[FStar.Tactics.exact (`emp_inames)] is:inames)
+  (p1 p2: slprop)
+  (sq: squash (p1 == p2))
+  requires p1
+  ensures p2 ** (Trade.trade #is p2 p1)
+{
+  Trade.rewrite_with_trade #is p1 p2
+}
+
+// inline_for_extraction noextract [@@noextract_to "krml"] let
+assume val write_expr_base_payload'
+  (xh1: header)
+: l2r_writer (vmatch_dep_proj2 (vmatch_synth rel_base synth_expr) xh1)
+    (serialize_nlist 
+      (count_payload xh1)
+      serialize_expr
+    )
+
+inline_for_extraction noextract [@@noextract_to "krml"]
+let write_expr_base_payload
+  (xh1: header)
+: l2r_writer (vmatch_dep_proj2 (vmatch_synth rel_base synth_expr) xh1)
+      (spec_serialize_recursive_payload serialize_expr_param xh1)
+= l2r_writer_ext
+    (write_expr_base_payload' xh1)
+    (spec_serialize_recursive_payload serialize_expr_param xh1)
+
+inline_for_extraction noextract [@@noextract_to "krml"]
+let mk_header
+  (lhs: U8.t)
+  (rhs: header_rhs lhs)
+: Tot header
+= (| lhs, rhs |)
+
+fn expr_base_get_header
+    (xl: expr_base_t)
+    (xh:
+      erased (dtuple2 header
+            (parse_recursive_payload_t expr
+                header
+                count_payload))
+    )
+requires
+      (vmatch_synth rel_base synth_expr xl xh)
+returns res: header
+ensures
+      (vmatch_synth rel_base synth_expr xl xh ** pure (res == dfst xh))
+{
+  unfold (vmatch_synth rel_base synth_expr xl xh);
+  let xh' = Ghost.hide (synth_expr xh);
+  rel_base_cases xl xh';
+  match xl {
+    EUPlus count payload -> {
+      let n = Ghost.hide (Plus?.n xh');
+      let l : Ghost.erased (nlist (Ghost.reveal n) expr) = Ghost.hide (Plus?.l xh');
+      Trade.rewrite_with_trade (rel_base xl xh') (rel_base_EUPlus count payload n () l);
+      unfold (vmatch_and_const (pure (eq2 #nat n (U8.v count))) (pts_to_serialized_with_perm (serialize_nlist n serialize_expr)) payload l);
+      fold (vmatch_and_const (pure (eq2 #nat n (U8.v count))) (pts_to_serialized_with_perm (serialize_nlist n serialize_expr)) payload l);
+      Trade.elim _ _;
+      fold (vmatch_synth rel_base synth_expr xl xh);
+      mk_header count (HUnit #count () ())
+    }
+    EValue v -> {
+      let v' : Ghost.erased U64.t = Value?._0 xh';
+      Trade.rewrite_with_trade (rel_base xl xh') (eq_as_slprop U64.t v v');
+      unfold (eq_as_slprop U64.t v v');
+      fold (eq_as_slprop U64.t v v');
+      Trade.elim _ _;
+      fold (vmatch_synth rel_base synth_expr xl xh);
+      mk_header 255uy (HValue () v)
+    }
+    EUMinus _ _ -> {
+      fold (vmatch_synth rel_base synth_expr xl xh);
+      mk_header 254uy (HUnit () ())
+    }
+  }
+}
+
+inline_for_extraction noextract [@@noextract_to "krml"]
+let write_expr_base_dtuple2 : l2r_writer (vmatch_synth rel_base synth_expr)
+  (serialize_dtuple2 serialize_header (spec_serialize_recursive_payload serialize_expr_param))
+= l2r_write_dtuple2_recip_explicit_header
+    write_header
+    expr_base_get_header
+    ()
+    write_expr_base_payload
+
+inline_for_extraction noextract [@@noextract_to "krml"]
+let write_expr_base' : l2r_writer #expr_base_t #expr rel_base #_ #_ (serialize_expr') =
+  l2r_write_synth_recip _ synth_expr synth_expr_recip write_expr_base_dtuple2
+
+let write_expr_base : l2r_writer #expr_base_t #expr rel_base #_ #_ (serialize_expr) =
+  [@@inline_let] let _ = parse_expr_eq () in
+  l2r_writer_ext write_expr_base' _
+
+(*
+inline_for_extraction
+let serialize_expr_base_EUPlus
+  (count: U8.t)
+  (n: Ghost.erased nat { n < 254 })
+: l2r_writer (vmatch_and_const (pure (U8.v count == Ghost.reveal n)) (pts_to_serialized_with_perm (serialize_nlist n serialize_expr))) serialize_expr
+= admit ()
+
+fn serialize_expr_base
+  (_: unit)
+: l2r_writer #expr_base_t #expr rel_base #_ #_ (serialize_expr)
+=
+  (xl: _)
+  (#xh: _)
+  (out: _)
+  (offset: _)
+  (#v: _)
+{
+  rel_base_cases xl xh;
+  match xl {
+    norewrite
+    EUPlus count s -> {
+      let n = Ghost.hide (Plus?.n xh);
+      let l = Ghost.hide (Plus?.l xh);
+      let sq = rel_base_eq_EUPlus xl xh count s n l () ();
+      rewrite_with_trade_squash _ _ sq;
+      admit ()
+    }
+    _ -> {
+      admit ()
+    }
+  }
+}
+
+
+(*
+inline_for_extraction noextract [@@noextract_to "krml"]
+fn serialize_expr_rec
+  (ser: l2r_writer rel (serializer_of_tot_serializer tot_serialize_expr))
+: l2r_writer #expr_t #expr rel #_ #_ (serializer_of_tot_serializer tot_serialize_expr)
+=
+  (xl: _)
+  (#xh: _)
+  (out: _)
+  (offset: _)
+  (#v: _)
+{
+  rel_cases xl xh;
+  rel_eq xl xh;
+  match xl {
+    norewrite
+    EPlus s -> {
+      let l = Ghost.hide (Plus?._0 xh);
+      Trade.rewrite_with_trade
+        (rel xl xh)
+        (nlist_match_slice0 rel (List.Tot.length l) s l);
+      l2r_write_nlist_as_slice 
+      admit ()
+    }
+    _ -> {
+      admit ()
+    }
   }
 }
