tests/pulse/ArithParse.Spec.fst
@@ -9,15 +9,13 @@ module U64 = FStar.UInt64
 module U8 = FStar.UInt8
 
 type expr =
-| Plus of (l: list expr { List.Tot.length l < 254 })
+| Plus: (n: nat) -> (sq: squash (n < 254)) -> (l: nlist n expr) -> expr
 | Minus of (expr & expr) // header 254
 | Value of U64.t // header 255
 
-let unit_as_uint64 = (x: U64.t { x == 0uL })
-inline_for_extraction noextract [@@noextract_to "krml"]
-let u_as_uint64 : unit_as_uint64 = 0uL
-
-let header_rhs (lhs: U8.t) = if lhs = 255uy then U64.t else unit_as_uint64
+type header_rhs (lhs: U8.t) =
+| HValue: (sq: squash (lhs = 255uy)) -> (v: U64.t) -> header_rhs lhs
+| HUnit: squash (lhs <> 255uy) -> (v: unit) -> header_rhs lhs
 
 let header = dtuple2 U8.t header_rhs
 
@@ -26,13 +24,13 @@ let parse_header_rhs_kind : parser_kind =
 
 let parse_header_rhs (lhs: U8.t) : Tot (parser parse_header_rhs_kind (header_rhs lhs)) =
       if lhs = 255uy
-      then weaken parse_header_rhs_kind parse_u64
-      else weaken parse_header_rhs_kind (parse_ret u_as_uint64)
+      then weaken parse_header_rhs_kind (parse_synth ( parse_u64) (HValue ()))
+      else weaken parse_header_rhs_kind (parse_synth (parse_empty) (HUnit ()))
 
 let tot_parse_header_rhs (lhs: U8.t) : Tot (tot_parser parse_header_rhs_kind (header_rhs lhs)) =
       if lhs = 255uy
-      then tot_weaken parse_header_rhs_kind tot_parse_u64
-      else tot_weaken parse_header_rhs_kind (tot_parse_ret u_as_uint64)
+      then tot_weaken parse_header_rhs_kind (tot_parse_synth (tot_parse_u64) (HValue ()))
+      else tot_weaken parse_header_rhs_kind (tot_parse_synth (tot_parse_empty) (HUnit ()))
 
 let tot_parse_header : tot_parser _ header =
   tot_parse_dtuple2 tot_parse_u8 tot_parse_header_rhs    
@@ -59,9 +57,9 @@ let count_payload (h: header) : Tot nat =
 let synth_expr (hp: parse_recursive_alt_t expr header count_payload) : Tot expr =
   let (| h, p |) = hp in
   match h with
-  | (| 255uy, v |) -> Value v
+  | (| 255uy, HValue _ v |) -> Value v
   | (| 254uy, _ |) -> let [v1; v2] = p in Minus (v1, v2)
-  | _ -> Plus p
+  | (| n, _ |) -> Plus (U8.v n) () p
 
 let parse_expr_kind = parse_recursive_kind parse_header_kind
 
@@ -70,6 +68,7 @@ let parse_expr_kind = parse_recursive_kind parse_header_kind
 let synth_expr_injective () : Lemma (synth_injective synth_expr) = ()
 #pop-options
 
+[@@Pulse.Lib.Pervasives.pulse_unfold]
 let parse_expr_param : parse_recursive_param = {
   t = expr;
   header = header;
@@ -82,18 +81,28 @@ let parse_expr_param : parse_recursive_param = {
 
 let tot_parse_expr = parse_recursive parse_expr_param
 
+let parse_expr = parser_of_tot_parser tot_parse_expr
+
+let parse_expr' =
+  (parse_header `parse_dtuple2` spec_parse_recursive_payload parse_expr_param parse_expr) `parse_synth` synth_expr
+
+let parse_expr_eq () : Lemma
+  (forall b. parse parse_expr' b == parse parse_expr b)
+= parse_header_eq ();
+  parse_recursive_eq_gen parse_expr_param _ parse_header
+
 let tot_serialize_header_rhs (lhs: U8.t) : tot_serializer (tot_parse_header_rhs lhs) =
   if lhs = 255uy
-  then tot_serialize_weaken parse_header_rhs_kind tot_serialize_u64
-  else tot_serialize_weaken parse_header_rhs_kind (tot_serialize_ret u_as_uint64 (fun _ -> ()))
+  then tot_serialize_weaken parse_header_rhs_kind (tot_serialize_synth _ (HValue ())  tot_serialize_u64 HValue?.v ())
+  else tot_serialize_weaken parse_header_rhs_kind (tot_serialize_synth _ (HUnit ())  tot_serialize_empty HUnit?.v ())
 
 let tot_serialize_header : tot_serializer tot_parse_header =
   tot_serialize_dtuple2 tot_serialize_u8 tot_serialize_header_rhs
 
 let serialize_header_rhs (lhs: U8.t) : serializer (parse_header_rhs lhs) =
   if lhs = 255uy
-  then serialize_weaken parse_header_rhs_kind serialize_u64
-  else serialize_weaken parse_header_rhs_kind (serialize_ret u_as_uint64 (fun _ -> ()))
+  then serialize_weaken parse_header_rhs_kind (serialize_synth _ (HValue ())  serialize_u64 HValue?.v ())
+  else serialize_weaken parse_header_rhs_kind (serialize_synth _ (HUnit ())  serialize_empty HUnit?.v ())
 
 let serialize_header : serializer parse_header =
   serialize_dtuple2 serialize_u8 serialize_header_rhs
@@ -102,9 +111,9 @@ let synth_expr_recip
   (x: expr)
 : Tot (parse_recursive_alt_t expr header count_payload)
 = match x with
-  | Value v -> (| (| 255uy, v |), [] |)
-  | Minus (v1, v2) -> (| (| 254uy, u_as_uint64 |), [v1; v2] |)
-  | Plus p -> (| (| U8.uint_to_t (List.Tot.length p), u_as_uint64 |), p |)
+  | Value v -> (| (| 255uy, HValue () v |), [] |)
+  | Minus (v1, v2) -> (| (| 254uy, HUnit () () |), [v1; v2] |)
+  | Plus n _ p -> (| (| U8.uint_to_t n, HUnit () () |), p |)
 
 let synth_expr_inverse () : Lemma (synth_inverse synth_expr synth_expr_recip) = ()
 
@@ -112,19 +121,19 @@ let rec level (x: expr) : Tot nat =
   match x with
   | Value _ -> 0
   | Minus (v1, v2) -> 1 + level v1 + level v2
-  | Plus l -> 1 + wf_list_sum l level
+  | Plus _ _ l -> 1 + wf_list_sum l level
 
 let level' (x: expr) : Tot nat =
   match x with
   | Value _ -> 0
   | Minus (v1, v2) -> 1 + level v1 + level v2
-  | Plus l -> 1 + list_sum level l
+  | Plus _ _ l -> 1 + list_sum level l
 
 let level_eq (x: expr) : Lemma
   (level x == level' x)
 = match x with
-  | Plus l ->
-    assert_norm (level (Plus l) == 1 + wf_list_sum l level);
+  | Plus _ _ l ->
+    assert_norm (level (Plus _ _ l) == 1 + wf_list_sum l level);
     wf_list_sum_eq level l
   | _ -> ()
 
@@ -134,7 +143,7 @@ let level_correct (x: expr) (n: nat) : Lemma
   (decreases x)
 = level_eq x;
   match x with
-  | Plus l ->
+  | Plus _ _ l ->
     forall_list_intro (has_level level (n - 1)) l (fun x ->
       list_sum_memP level l x
     )
@@ -149,3 +158,16 @@ let serialize_expr_param : serialize_recursive_param parse_expr_param = {
 }
 
 let tot_serialize_expr : tot_serializer tot_parse_expr = serialize_recursive serialize_expr_param
+
+let serialize_expr : serializer parse_expr = serializer_of_tot_serializer tot_serialize_expr
+
+let serialize_expr' : serializer parse_expr' =
+  serialize_synth
+    _
+    synth_expr
+    (serialize_dtuple2
+      serialize_header
+      (spec_serialize_recursive_payload serialize_expr_param)
+    )
+    synth_expr_recip
+    ()
